Coq semantics updated for expressions

formal_semantics/semantique.v
@@ -15,7 +15,8 @@ Definition fsub := b64_minus mode_NE.
 Definition fmult := b64_mult mode_NE.
 Definition fdiv := b64_div mode_NE.
 Definition fopp := b64_opp.
-Definition fzero : binary64 := B754_zero 53 1024 false. (* or true? *)
+Definition fzero : binary64 := B754_zero 53 1024 false.
+
 Definition fabs := b64_abs.
 Definition flt f1 f2 :=
   match b64_compare f1 f2 with
@@ -27,15 +28,26 @@ Definition feq f1 f2 :=
   | Some Eq => true
   | _ => false
   end.
+Definition fne f1 f2 :=
+  match b64_compare f1 f2 with
+  | Some Ne => true
+  | _ => false
+  end.
 Definition fgt f1 f2 :=
   match b64_compare f1 f2 with
   | Some Gt => true
+  | _ => false
+  end.
+Definition fge f1 f2 :=
+  match b64_compare f1 f2 with
+  | Some Ge => true
   | _ => false
   end.
 Definition fmin f1 f2 :=
   if flt f1 f2 then f1 else f2.
 Definition fmax f1 f2 :=
   if flt f1 f2 then f2 else f1.
+
 
 (* Similar to CompCert's implementation *)
 Definition ZofB64 (f: binary64): option Z :=
@@ -60,35 +72,45 @@ Qed.
 
 Definition B64ofZ (z:Z) := binary_normalize prec emax Hprec Hprec_emax mode_NE z 0 false.
 
-Definition is_integer (f: binary64) :=
-  match f with
-  | B754_finite _ _ s m (Zpos e) _ => true
-  | B754_finite _ _ s m (Zneg e) _ => (((Zpos m) mod Z.pow radix2 (Zpos e)) =? 0)%Z
-  | B754_zero _ _ b => true
-  | _ => false
-  end.
+Definition fone := B64ofZ (1%Z).
 
-Definition valid_int_between (f: binary64) (l: Z) (u: Z) :=
-  andb (is_integer f) (match ZofB64 f with
-  | Some fz => andb (l <=? fz)%Z (fz <? u)%Z
-  | None => false
-  end).
+Definition fandb f1 f2 :=
+  andb (fne f1 fzero) (fne f2 fzero).
+
+Definition forb f1 f2 :=
+  orb (fne f1 fzero) (fne f2 fzero).
+
+Definition float_of_bool (b:bool) :=
+  if b then fone else fzero.
+
+
+
+(* Definition is_integer (f: binary64) := *)
+(*   match f with *)
+(*   | B754_finite _ _ s m (Zpos e) _ => true *)
+(*   | B754_finite _ _ s m (Zneg e) _ => (((Zpos m) mod Z.pow radix2 (Zpos e)) =? 0)%Z *)
+(*   | B754_zero _ _ b => true *)
+(*   | _ => false *)
+(*   end. *)
+
+(* Definition valid_int_between (f: binary64) (l: Z) (u: Z) := *)
+(*   andb (is_integer f) (match ZofB64 f with *)
+(*   | Some fz => andb (l <=? fz)%Z (fz <? u)%Z *)
+(*   | None => false *)
+(*   end). *)
 
 (* checks that f is an integer, and between 0 and u *)
 Definition valid_integer_access (f: binary64) (u: N) : option nat :=
-  if is_integer f then
     match ZofB64 f with
     | Some fz => if (andb (0 <=? fz)%Z (fz <? (Z.of_N u))%Z) then Some (Z.to_nat fz) else None
     | _ => None
-    end
-  else None.
+    end.
 
 Lemma valid_integer_access_spec : forall f s n,
   valid_integer_access f s = Some n -> n < (N.to_nat s).
 Proof.
   intros.
   unfold valid_integer_access in H.
-  destruct (is_integer f); try discriminate.
   destruct (ZofB64 f); try discriminate.
   destruct ((0 <=? z)%Z && (z <? Z.of_N s)%Z)%bool eqn:Eq; try discriminate.
   rewrite Bool.andb_true_iff in Eq; destruct Eq.
@@ -118,16 +140,12 @@ Definition variable := string.
 Definition table_size := N.
 
 
-Inductive type :=
-| TBool
-| TFloat.
 
 Inductive envtypes :=
-| TScalar : type -> envtypes
-| TTable : type -> envtypes.
+| TScalar
+| TTable.
 
 Inductive values :=
-| Bool : bool ->  values
 | Float : binary64 -> values
 | Undef : values.
 
@@ -137,17 +155,13 @@ Inductive envvalues :=
 
 (* Contrary to the paper, we separated usual binary operators from
 functions *)
-Inductive logicop := | And | Or.
+(* Inductive boolop := | And | Or | Lt | Eq. *)
 
-Inductive compop :=
-| Lt
-| Eq.
-
-Inductive arithop :=
-| Add
-| Sub
-| Mul
-| Div.
+(* Inductive arithop := *)
+(* | Add *)
+(* | Sub *)
+(* | Mul *)
+(* | Div. *)
 
 (* Functions are handled in an ad-hoc manner to simplify the
 formalization and due to the finite and small number of defined
@@ -159,6 +173,7 @@ Inductive func1 :=
 
 (* Functions of arity 2 *)
 Inductive func2 :=
+| And | Or | Lt | Eq | Add | Sub | Mul | Div
 | Min | Max.
 
 
@@ -169,9 +184,8 @@ Inductive expression :=
 | X : expression
 | Var : variable -> expression
 | UNeg : expression -> expression
-| Logic : logicop -> expression -> expression -> expression
-| Comp : compop -> expression -> expression -> expression
-| Arith : arithop -> expression -> expression -> expression
+(* | Boolop : boolop -> expression -> expression -> expression *)
+(* | Arith : arithop -> expression -> expression -> expression *)
 | FunCall1 : func1 -> expression -> expression
 | FunCall2 : func2 -> expression -> expression -> expression
 | TableAccess : variable -> expression -> expression.
@@ -208,73 +222,122 @@ Definition type_environment := partial_map envtypes.
 (* Semantics of some functions and binary operators *)
 (****************************************************)
 
-Definition add (l:values) (r:values) : option values :=
+Definition add (l:values) (r:values) : values :=
   match l, r with
-  | Undef, Undef => Some Undef
-  | Undef, Float f2 => Some (Float f2)
-  | Float f1, Undef => Some (Float f1)
-  | Float f1, Float f2  => Some (Float (fadd f1 f2))
-  | _, _ => None
+  | Undef, Undef =>  Undef
+  | Undef, Float f2 => Float f2
+  | Float f1, Undef => Float f1
+  | Float f1, Float f2  => Float (fadd f1 f2)
   end.
 
-Definition sub (l:values) (r:values) : option values :=
+Definition sub (l:values) (r:values) : values :=
   match l, r with
-  | Undef, Undef => Some Undef
-  | Undef, Float f2 => Some (Float (fopp f2))
-  | Float f1, Undef => Some (Float f1)
-  | Float f1, Float f2  => Some (Float (fsub f1 f2))
-  | _, _ => None
+  | Undef, Undef => Undef
+  | Undef, Float f2 => Float (fopp f2)
+  | Float f1, Undef => Float f1
+  | Float f1, Float f2  => Float (fsub f1 f2)
   end.
 
-Definition mul (l:values) (r:values) : option values :=
+Definition mul (l:values) (r:values) : values :=
   match l, r with
-  | Undef, Undef => Some Undef
-  | Undef, Float f2 => Some (Float fzero)
-  | Float f1, Undef => Some (Float fzero)
-  | Float f1, Float f2  => Some (Float (fmult f1 f2))
-  | _, _ => None
+  | Undef, _ | _, Undef => Undef
+  | Float f1, Float f2  => Float (fmult f1 f2)
   end.
 
-Definition div (l: values) (r: values) : option values :=
+Definition div (l: values) (r: values) : values :=
   match l, r with
-  | Undef, Undef => Some Undef
-  | Float f1, Undef => Some Undef
-  | Float f1, Float (B754_zero _ _ _) => Some Undef
-  | Undef, Float f2 => Some (Float fzero)
-  | Float f1, Float f2 => Some (Float (fdiv f1 f2))
-  | _, _ => None
+  | Undef, _ | _, Undef  => Undef
+  | Float f1, Float (B754_zero _ _ _) => Float fzero
+  | Float f1, Float f2 => Float (fdiv f1 f2)
   end.
 
-Definition and (l: values) (r: values) : option values :=
+
+Definition and (l: values) (r: values) : values :=
   match l, r with
-  | Undef, _ => Some Undef
-  | _, Undef => Some Undef
-  | Bool b1, Bool b2 => Some (Bool (andb b1 b2))
-  | _, _ => None
+  | Undef, _ | _, Undef  => Undef
+  | Float f1, Float f2 => Float (float_of_bool (fandb f1 f2))
   end.
 
-Definition or (l: values) (r: values) : option values :=
+Definition or (l: values) (r: values) : values :=
   match l, r with
-  | Undef, _ => Some Undef
-  | _, Undef => Some Undef
-  | Bool b1, Bool b2 => Some (Bool (orb b1 b2))
-  | _, _ => None
+  | Undef, _ | _, Undef => Undef
+  | Float f1, Float f2 => Float (float_of_bool (forb f1 f2))
   end.
 
-Definition lt (l: values) (r: values) : option values :=
+Definition lt (l: values) (r: values) : values :=
   match l, r with
-  | Undef, _ => Some Undef
-  | _, Undef => Some Undef
-  | Float f1, Float f2 => Some (Bool (flt f1 f2))
-  | _, _ => None
+  | Undef, _ | _, Undef => Undef
+  | Float f1, Float f2 => Float (float_of_bool (flt f1 f2))
   end.
 
-Definition eq (l: values) (r: values) : option values :=
+Definition eq (l: values) (r: values) : values :=
   match l, r with
-  | Undef, _ => Some Undef
-  | _, Undef => Some Undef
-  | Float f1, Float f2 => Some (Bool (feq f1 f2))
-  | _, _ => None
+  | Undef, _ | _, Undef => Undef
+  | Float f1, Float f2 => Float (float_of_bool (feq f1 f2))
+  end.
+
+Definition min (l: values) (r: values) : values :=
+  match l, r with
+  | Undef, Undef => Float fzero
+  | Float f1, Undef => Float (fmin f1 fzero)
+  | Undef, Float f2 => Float (fmin fzero f2)
+  | Float f1, Float f2 => Float (fmin f1 f2)
+  end.
+
+Definition max (l: values) (r: values) : values :=
+  match l, r with
+  | Undef, Undef => Float fzero
+  | Float f1, Undef => Float (fmax f1 fzero)
+  | Undef, Float f2 => Float (fmax fzero f2)
+  | Float f1, Float f2 => Float (fmax f1 f2)
+  end.
+
+Definition round (v : values) : values :=
+  match v with
+  | Undef => Undef
+  | Float f =>
+    (* FIXME: there should be a round here, but I haven't found the
+    corresponding Flocq definition yet. We could always cast to
+    integers and back... *)
+    Float f
+  end.
+
+Definition inf (v: values) : values :=
+  match v with
+  | Undef => Undef
+  (* FIXME: inf missing *)
+  | Float f => Float f
+  end.
+
+Definition abs (v: values) : values :=
+  match v with
+  | Undef => Undef
+  | Float f => Float (fabs f)
+  end.
+
+
+Definition gtzero (v: values) : values :=
+  match v with
+  | Undef => Undef
+  | Float f => Float (float_of_bool (fgt f fzero))
+  end.
+
+Definition gtezero (v: values) : values :=
+  match v with
+  | Undef => Undef
+  | Float f => Float (float_of_bool (fge f fzero))
+  end.
+
+Definition null (v: values) : values :=
+  match v with
+  | Undef => Undef
+  | Float f => Float (float_of_bool (feq f fzero))
+  end.
+
+Definition present (v: values) : values :=
+  match v with
+  | Undef => Float (float_of_bool false)
+  | Float f => Float (float_of_bool true)
   end.
 
 Definition scalar_of_envvalue (e : envvalues) : option values :=
@@ -291,9 +354,10 @@ Fixpoint eval (Omega:environment) (e:expression) : option values :=
   | Value v => Some v
   | If cond t f =>
     match eval Omega cond with
-    | Some (Bool true) => eval Omega t
-    | Some (Bool false) => eval Omega f
-    | Some (Undef) => Some Undef
+    | Some (Float c) =>
+      if feq c fzero then eval Omega f else eval Omega t
+    | Some Undef =>
+      Some Undef
     | _ => None
     end
   | X =>
@@ -308,103 +372,44 @@ Fixpoint eval (Omega:environment) (e:expression) : option values :=
     end
   | UNeg e =>
     match eval Omega e with
-    | Some (Bool b) => Some (Bool (negb b))
+    | Some (Float f) => Some (Float (fsub fone f))
     | Some Undef => Some Undef
     | _ => None
     end
-  | Logic o e1 e2 =>
-    let ee1 := eval Omega e1 in
-    let ee2 := eval Omega e2 in
+  | FunCall1 o arg1 =>
+    match eval Omega arg1 with
+    | Some v =>
+      Some
+        (match o with
+         | Round => round v
+         | Inf => inf v
+         | Abs => abs v
+         | Gtzero => gtzero v
+         | Gtezero => gtezero v
+         | Null => null v
+         | Present => present v
+         end
+        )
+    | _ => None
+    end
+  | FunCall2 o arg1 arg2 =>
+    let ee1 := eval Omega arg1 in
+    let ee2 := eval Omega arg2 in
     match ee1, ee2 with
     | Some v1, Some v2 =>
-      match o with
-      | And => and v1 v2
-      | Or => or v1 v2
-      end
-    | _, _ => None
-    end
-  | Comp c e1 e2 =>
-    let ee1 := eval Omega e1 in
-    let ee2 := eval Omega e2 in
-    match ee1, ee2 with
-    | Some v1, Some v2 =>
-      match c with
-      | Lt => lt v1 v2
-      | Eq => eq v1 v2
-      end
-    | _, _ => None
-    end
-  | Arith op e1 e2 =>
-    let ee1 := eval Omega e1 in
-    let ee2 := eval Omega e2 in
-    match ee1, ee2 with
-    | Some v1, Some v2 => match op with
-                          | Add => add v1 v2
-                          | Sub => sub v1 v2
-                          | Mul => mul v1 v2
-                          | Div => div v1 v2
-                          end
-    | _, _ => None
-    end
-  | FunCall1 Round arg1 =>
-    match eval Omega arg1 with
-    | Some (Float f) => Some (Float f)
-    (* FIXME: there should be a round here, but I haven't found the
-    corresponding Flocq definition yet. We could always cast to
-    integers and back... *)
-    | Some Undef => Some (Float fzero)
-    | _ => None
-    end
-  | FunCall1 Inf arg1 =>
-    match eval Omega arg1 with
-    | Some (Float f) => Some (Float f)
-    (* FIXME: Inf missing in the float computation *)
-    | Some Undef => Some (Float fzero)
-    | _ => None
-    end
-  | FunCall1 Abs arg1 =>
-    match eval Omega arg1 with
-    | Some (Float f) => Some (Float (fabs f))
-    | Some Undef => Some Undef
-    | _ => None
-    end
-  | FunCall1 Gtzero arg1 =>
-    match eval Omega arg1 with
-    | Some (Float f) => Some (Bool (fgt f fzero))
-    | Some Undef => Some Undef
-    | _ => None
-    end
-  | FunCall1 Gtezero arg1 =>
-    match eval Omega arg1 with
-    | Some (Float f) => Some (Bool (orb (fgt f fzero) (feq f fzero)))
-    | Some Undef => Some Undef
-    | _ => None
-    end
-  | FunCall1 Null arg1 =>
-    match eval Omega arg1 with
-    | Some Undef => Some Undef
-    | Some (Float f) => Some (Bool (feq f fzero))
-    | Some (Bool b) => Some (Bool (Bool.eqb b false))
-    | _ => None
-    end
-  | FunCall1 Present arg1 =>
-    match eval Omega arg1 with
-    | Some Undef => Some (Bool false)
-    | Some _ => Some (Bool true)
-    | _ => None
-    end
-  | FunCall2 Min arg1 arg2 =>
-    match eval Omega arg1, eval Omega arg2 with
-    | Some (Float f1), Some (Float f2) => Some (Float (fmin f1 f2))
-    | Some Undef, _ => Some Undef
-    | _, Some Undef => Some Undef
-    | _, _ => None
-    end
-  | FunCall2 Max arg1 arg2 =>
-    match eval Omega arg1, eval Omega arg2 with
-    | Some (Float f1), Some (Float f2) => Some (Float (fmax f1 f2))
-    | Some Undef, _ => Some Undef
-    | _, Some Undef => Some Undef
+      Some
+        (match o with
+         | And => and v1 v2
+         | Or  => or  v1 v2
+         | Lt  => lt  v1 v2
+         | Eq  => eq  v1 v2
+         | Add => add v1 v2
+         | Sub => sub v1 v2
+         | Mul => mul v1 v2
+         | Div => div v1 v2
+         | Min => min v1 v2
+         | Max => max v1 v2
+         end)
     | _, _ => None
     end
   | TableAccess var index =>
@@ -412,11 +417,13 @@ Fixpoint eval (Omega:environment) (e:expression) : option values :=
     | Some (Float f) =>
       match Omega var with
       | Some (VTable values size) =>
-        match valid_integer_access f size with
-        | Some index =>
-          Some (List.nth index values Undef)
-        | None => Some Undef
-        end
+        if flt f fzero then Some (Float fzero)
+        else
+          match valid_integer_access f size with
+          | Some index =>
+            Some (List.nth index values Undef)
+          | None => Some Undef
+          end
       | Some (VScalar _) => None
       | None => Some Undef
       end
@@ -432,81 +439,54 @@ Fixpoint eval (Omega:environment) (e:expression) : option values :=
 (************************************)
 (* Typing jugement for expressions  *)
 (************************************)
-Inductive well_typed : type_environment -> expression -> type -> Prop :=
-| WTBool : forall Gamma b, well_typed Gamma (Value (Bool b)) TBool
-| WTFloat : forall Gamma f, well_typed Gamma (Value (Float f)) TFloat
-| WTUndef : forall Gamma tau, well_typed Gamma (Value Undef) tau
-| WTVar : forall Gamma x tau, Gamma(x) = Some (TScalar tau) -> well_typed Gamma (Var x) tau
-| WTVarUndef : forall Gamma x tau, Gamma(x) = None -> well_typed Gamma (Var x) tau
-| WTComp : forall Gamma compop e1 e2, well_typed Gamma e1 TFloat ->
-                                 well_typed Gamma e2 TFloat ->
-                                 well_typed Gamma (Comp compop e1 e2) TBool
-| WTLogic : forall Gamma logop e1 e2, well_typed Gamma e1 TBool ->
-                                 well_typed Gamma e2 TBool ->
-                                 well_typed Gamma (Logic logop e1 e2) TBool
-| WTUneg : forall Gamma e, well_typed Gamma e TBool -> well_typed Gamma (UNeg e) TBool
-| WTIf : forall Gamma cond tr fa tau, well_typed Gamma cond TBool ->
-                           well_typed Gamma tr tau ->
-                           well_typed Gamma fa tau ->
-                           well_typed Gamma (If cond tr fa) tau
-| WTArith : forall Gamma op e1 e2, well_typed Gamma e1 TFloat ->
-                             well_typed Gamma e2 TFloat ->
-                             well_typed Gamma (Arith op e1 e2) TFloat
-| WTIndex : forall Gamma tabvar index tabtau,
-    Gamma(tabvar) = Some (TTable tabtau) ->
-    well_typed Gamma index TFloat ->
-    well_typed Gamma (TableAccess tabvar index) tabtau
-| WTFuncFloat1Bool :
-    forall Gamma f arg,
-      f = Gtzero \/ f = Gtezero ->
-      well_typed Gamma arg TFloat ->
-      well_typed Gamma (FunCall1 f arg) TBool
-| WTFuncFloat1Float :
-    forall Gamma f arg,
-      f = Round \/ f = Inf \/ f = Abs ->
-      well_typed Gamma arg TFloat ->
-      well_typed Gamma (FunCall1 f arg) TFloat
-| WTFuncFloat2 :
-    forall Gamma f arg1 arg2,
-      f = Min \/ f = Max ->
-      well_typed Gamma arg1 TFloat ->
-      well_typed Gamma arg2 TFloat ->
-      well_typed Gamma (FunCall2 f arg1 arg2) TFloat
-| WTFuncTop1Bool :
-    forall Gamma tau f arg,
-      f = Null \/ f = Present ->
-      well_typed Gamma arg tau ->
-      well_typed Gamma (FunCall1 f arg) TBool.
+Inductive well_formed : type_environment -> expression -> Prop :=
+| WTFloat : forall Gamma f, well_formed Gamma (Value (Float f))
+| WTUndef : forall Gamma, well_formed Gamma (Value Undef)
+| WTVarUndef : forall Gamma x, Gamma(x) = None -> well_formed Gamma (Var x)
+| WTVar : forall Gamma x, Gamma(x) = Some TScalar -> well_formed Gamma (Var x)
+| WTIndexUndef : forall Gamma x e, Gamma(x) = None -> well_formed Gamma e -> well_formed Gamma (TableAccess x e)
+| WTIndex : forall Gamma tabvar index,
+    Gamma(tabvar) = Some TTable ->
+    well_formed Gamma index ->
+    well_formed Gamma (TableAccess tabvar index)
+| WTConditional : forall Gamma cond tr fa,
+    well_formed Gamma cond ->
+    well_formed Gamma tr ->
+    well_formed Gamma fa ->
+    well_formed Gamma (If cond tr fa)
+| WTfunc1 : forall Gamma f arg,
+    well_formed Gamma arg ->
+    well_formed Gamma (FunCall1 f arg)
+| WTfunc2 : forall Gamma f a1 a2,
+    well_formed Gamma a1 ->
+    well_formed Gamma a2 ->
+    well_formed Gamma (FunCall2 f a1 a2).
 
-Inductive value_of_type : values -> type -> Prop :=
-| VoBool : forall b, value_of_type (Bool b) TBool
-| VoFloat : forall f, value_of_type (Float f) TFloat
-| VoUndef : forall tau, value_of_type Undef tau.
+(* Inductive value_of_type : values -> type -> Prop := *)
+(* | VoBool : forall b, value_of_type (Bool b) TBool *)
+(* | VoFloat : forall f, value_of_type (Float f) TFloat *)
+(* | VoUndef : forall tau, value_of_type Undef tau. *)
 
-Hint Constructors value_of_type.
+(* Hint Constructors value_of_type. *)
 
 (***********************************************************************************)
 (* These definitions specify how type and evaluation environnements can be related *)
 (***********************************************************************************)
 Definition related_envs_some_scalar (Gamma: type_environment) (Omega: environment) :=
-  forall (s: string) ,
-  forall tau, Gamma s = Some (TScalar tau) ->
-         exists v, Omega s = Some (VScalar v) /\ value_of_type v tau.
+  forall (s: variable), Gamma s = Some TScalar ->
+                   exists v, Omega s = Some (VScalar v).
 
 Definition related_envs_some_tbl (Gamma: type_environment) (Omega: environment) :=
-  forall (s: string),
-    forall tau, Gamma s = Some (TTable tau) -> exists v size, Omega s = Some (VTable v size) /\ List.Forall (fun el => value_of_type el tau) v /\ (N.to_nat size) = List.length v.
-(* I don't know if we need size = size', or if we can prove size = size' or sth... *)
+  forall (s: string), Gamma s = Some TTable -> exists v size, Omega s = Some (VTable v size) /\ (N.to_nat size) = List.length v.
 
 Definition related_envs_none (Gamma: type_environment) (Omega: environment) :=
   forall (s: string), Gamma s = None -> Omega s = None.
 
-
-Definition value_of_type_sound :
-  forall v tau Gamma, value_of_type v tau -> well_typed Gamma (Value v) tau.
-Proof.
-  intros ? ? ? VoT; inversion VoT; subst; constructor; eauto.
-Qed.
+(* Definition value_of_type_sound : *)
+(*   forall v tau Gamma, value_of_type v tau -> well_formed Gamma (Value v) tau. *)
+(* Proof. *)
+(*   intros ? ? ? VoT; inversion VoT; subst; constructor; eauto. *)
+(* Qed. *)
 
 
 (***************************************************)
@@ -516,56 +496,38 @@ Theorem soundness_expr :
   forall Gamma Omega, related_envs_some_scalar Gamma Omega ->
                  related_envs_some_tbl Gamma Omega ->
                  related_envs_none Gamma Omega ->
-                 forall e tau, well_typed Gamma e tau -> exists v, eval Omega e = Some v /\ value_of_type v tau.
+                 forall e, well_formed Gamma e -> exists v, eval Omega e = Some v.
 Proof.
   intros Gamma Omega rGOSS rGOST rGON.
   induction e; intros ; inversion H; subst; simpl; eauto.
-  - destruct (IHe1 TBool H4) as [v [IHe1e IHe1vt]]; clear IHe1; rewrite IHe1e.
+  - destruct (IHe1 H4) as [v IHe1e]; rewrite IHe1e.
     destruct v.
-    + destruct b; eauto.
-    + inversion IHe1vt.
+    + destruct feq; eauto.
     + eauto.
-  - destruct (rGOSS _ _ H2) as [v0 [O_eq v0_ty]]; rewrite O_eq; simpl; eauto.
   - specialize (rGON _ H2); rewrite rGON; eauto.
-  - destruct (IHe _ H2) as [v [O_eq v_ty]]; rewrite O_eq; simpl.
-    inversion v_ty; subst; eauto.
-  - destruct (IHe1 _ H5) as [v1 [IHe1v IHe1t]]; clear IHe1; rewrite IHe1v.
-    destruct (IHe2 _ H6) as [v2 [IHe2v IHe2t]]; clear IHe2; rewrite IHe2v.
-    inversion IHe1t as [? | f1 | ? ]; subst;
-      inversion IHe2t as [? | f2 | ?]; subst; destruct l; simpl; eauto.
-  - destruct (IHe1 _ H5) as [v1 [IHe1v IHe1t]]; clear IHe1; rewrite IHe1v.
-    destruct (IHe2 _ H6) as [v2 [IHe2v IHe2t]]; clear IHe2; rewrite IHe2v.
-    inversion IHe1t as [? | f1 | ? ]; subst;
-      inversion IHe2t as [? | f2 | ?]; subst; destruct c; simpl; eauto.
-  - destruct (IHe1 _ H5) as [v1 [IHe1v IHe1t]]; clear IHe1; rewrite IHe1v.
-    destruct (IHe2 _ H6) as [v2 [IHe2v IHe2t]]; clear IHe2; rewrite IHe2v.
-    inversion IHe1t as [? | f1 | ? ]; subst;
-      inversion IHe2t as [? | f2 | ?]; subst; destruct a; simpl; eauto.
-    destruct f2; eauto.
-  - destruct (IHe _ H5) as [v [O_eq v_ty]]; rewrite O_eq; simpl.
-    destruct H3; subst; inversion v_ty; eauto.
-  - destruct (IHe _ H5) as [v [O_eq v_ty]]; rewrite O_eq; simpl.
-    destruct H3 as [? | [? | ?]]; subst; inversion v_ty; eauto.
-  - destruct (IHe _ H5) as [v [O_eq v_ty]]; rewrite O_eq; simpl.
-    destruct H3; subst; inversion v_ty; eauto.
-  - destruct (IHe1 _ H6) as [v1 [IHe1v IHe1t]]; clear IHe1; rewrite IHe1v.
-    destruct (IHe2 _ H7) as [v2 [IHe2v IHe2t]]; clear IHe2; rewrite IHe2v.
-    inversion IHe1t as [? | f1 | ? ]; subst;
-      inversion IHe2t as [? | f2 | ?]; subst; destruct H4; subst; simpl; eauto.
-  - destruct (IHe _ H5) as [ve [O_eq v_ty]]; rewrite O_eq; simpl.
-    inversion v_ty; subst; eauto.
-    specialize (rGOST _ _ H3).
-    destruct rGOST as [v0 [s0 [Ov0_eq [Altau v0_eq]]]].
+  - destruct (rGOSS _ H2) as [v0 O_eq]; rewrite O_eq; simpl; eauto.
+  - destruct (IHe H2) as [v O_eq]; rewrite O_eq; simpl.
+    destruct f; simpl; eauto.
+  - destruct (IHe1 H3) as [v1 IHe1v]; clear IHe1; rewrite IHe1v.
+    destruct (IHe2 H5) as [v2 IHe2v]; clear IHe2; rewrite IHe2v.
+    destruct f; simpl; eauto.
+  - destruct (IHe H4) as [ve O_eq]; rewrite O_eq; simpl.
+    specialize (rGON _ H3); rewrite rGON.
+    eexists Undef; destruct ve; eauto.
+  - destruct (IHe H4) as [ve O_eq]; rewrite O_eq; simpl.
+    specialize (rGOST _ H3).
+    destruct rGOST as [v0 [s0 [Ov0_eq length]]].
     rewrite Ov0_eq.
-    destruct (valid_integer_access f _) eqn:VIA.
-    + rewrite List.Forall_forall in Altau.
-      pose proof valid_integer_access_spec _ _ _ VIA.
-      rewrite v0_eq in H0.
+    destruct ve; eauto.
+    destruct flt; eauto.
+    destruct (valid_integer_access _ _) eqn:VIA.
+    + pose proof valid_integer_access_spec _ _ _ VIA.
+      rewrite length in H0.
       pose proof (List.nth_In _ Undef H0).
-      specialize (Altau _ H1).
       eauto.
     + eauto.
 Qed.
+
 
 Require Import String.
 Open Scope string_scope.
@@ -635,16 +597,16 @@ Fixpoint exec_program (Omega: cmd_environment) (p: program) : option cmd_environ
 (* Typing judgment for commands and programs *)
 (*********************************************)
 
-Inductive well_typed_cmd : type_environment -> command -> type_environment -> Prop :=
-| WTCAssign : forall Gamma var expr tau, well_typed Gamma expr tau -> well_typed_cmd Gamma (Assign var expr) (upd_map _ var  (TScalar tau) Gamma)
+Inductive well_formed_cmd : type_environment -> command -> type_environment -> Prop :=
+| WTCAssign : forall Gamma var expr tau, well_formed Gamma expr tau -> well_formed_cmd Gamma (Assign var expr) (upd_map _ var  (TScalar tau) Gamma)
 | WTCAssignTable : forall Gamma var tabsize expr tau,
     tabsize <> N0 ->
-    well_typed (upd_map _ "X"%string (TScalar TFloat) Gamma) expr tau -> well_typed_cmd Gamma (TableAssign var tabsize expr) (upd_map _ var (TTable tau) Gamma)
-| WTCCond : forall Gamma cond err, well_typed Gamma cond TBool -> well_typed_cmd Gamma (Verif cond err) Gamma.
+    well_formed (upd_map _ "X"%string (TScalar TFloat) Gamma) expr tau -> well_formed_cmd Gamma (TableAssign var tabsize expr) (upd_map _ var (TTable tau) Gamma)
+| WTCCond : forall Gamma cond err, well_formed Gamma cond TBool -> well_formed_cmd Gamma (Verif cond err) Gamma.
 
-Inductive well_typed_prog : type_environment -> program -> type_environment -> Prop :=
-| WTPnil : forall Gamma, well_typed_prog Gamma nil Gamma
-| WTPcons : forall Gamma c p' Gamma' Gamma'', well_typed_cmd Gamma c Gamma' -> well_typed_prog Gamma' p' Gamma'' -> well_typed_prog Gamma (c :: p') Gamma''.
+Inductive well_formed_prog : type_environment -> program -> type_environment -> Prop :=
+| WTPnil : forall Gamma, well_formed_prog Gamma nil Gamma
+| WTPcons : forall Gamma c p' Gamma' Gamma'', well_formed_cmd Gamma c Gamma' -> well_formed_prog Gamma' p' Gamma'' -> well_formed_prog Gamma (c :: p') Gamma''.
 
 (******************************************************************)
 (* Related environments lifted to evaluation context for commands *)
@@ -745,7 +707,7 @@ Lemma exec_tbl_acc:
     related_envs_some_scalar Gamma Omega ->
     related_envs_some_tbl Gamma Omega ->
     related_envs_none Gamma Omega ->
-    well_typed (upd_map _ "X"%string (TScalar TFloat) Gamma) e tau ->
+    well_formed (upd_map _ "X"%string (TScalar TFloat) Gamma) e tau ->
     forall n acc,
     bound >= n ->
     exists vals, exec_tbl Omega bound e n acc = Some (List.rev acc ++ vals)%list /\ List.length vals = S n /\
@@ -791,7 +753,7 @@ Qed.
 (**********************************)
 Theorem soundness_cmd :
   forall Gamma Omega c Gamma',
-    well_typed_cmd Gamma c Gamma' ->
+    well_formed_cmd Gamma c Gamma' ->
     related_envs Gamma Omega ->
     exists Omega', exec Omega c = Some Omega' /\ (related_envs Gamma' Omega').
 Proof.
@@ -840,7 +802,7 @@ Qed.
 (**********************************)
 Theorem soundness_prog :
   forall p Gamma Omega Gamma',
-    well_typed_prog Gamma p Gamma' ->
+    well_formed_prog Gamma p Gamma' ->
     related_envs Gamma Omega ->
     exists Omega', exec_program Omega p = Some Omega' /\ (related_envs Gamma' Omega').
 Proof.
@@ -854,7 +816,7 @@ Qed.
 
 Theorem soundness_prog_starting_from_scratch:
   forall p Gamma,
-    well_typed_prog (fun _ => None) p Gamma ->
+    well_formed_prog (fun _ => None) p Gamma ->
     exists Omega, exec_program (Some (fun _ => None)) p = Some Omega /\ related_envs Gamma Omega.
 Proof.
   intros.
